Semantic/FsubNext/Denotation.lean
@@ -1,3 +1,0 @@
-import Semantic.FsubNext.Denotation.Core
-import Semantic.FsubNext.Denotation.Rebind
-import Semantic.FsubNext.Denotation.Retype
